src/ShouldBuild.v
@@ -5,6 +5,8 @@ From Perennial Require Import program_logic.crash_inv.
 
 From Perennial.go_lang Require Import
      adequacy total_adequacy lib.spin_lock.
+From Perennial.go_lang.examples Require Import
+     proof.append_log_proof.
 (* goose deep output *)
 From Perennial.go_lang.examples Require Import
      goose_unittest append_log wal mailserver simpledb logging2 rfc1813.
