src/go_lang/examples/proof/append_log_proof.v
@@ -1,0 +1,34 @@
+From iris.proofmode Require Import coq_tactics reduction.
+From Perennial.go_lang.examples Require Import append_log.
+From Perennial.go_lang Require Import basic_triples.
+From Perennial.go_lang Require Import slice encoding.
+From Perennial.go_lang Require Import ffi.disk.
+From Perennial.go_lang Require Import ffi.disk_prelude.
+Import uPred.
+
+Section heap.
+Context `{!heapG Σ}.
+Context `{!diskG Σ}.
+Implicit Types P Q : iProp Σ.
+Implicit Types Φ : val → iProp Σ.
+Implicit Types Δ : envs (uPredI (iResUR Σ)).
+Implicit Types v : val.
+Implicit Types z : Z.
+Implicit Types s : Slice.t.
+Implicit Types stk : stuckness.
+
+Definition is_hdr (sz disk_sz: u64): iProp Σ :=
+  ∃ b, 0 d↦ b ∗
+       ⌜take 8 (Block_to_vals b) = u64_le_bytes sz⌝ ∗
+       ⌜take 8 (drop 8 (Block_to_vals b)) = u64_le_bytes disk_sz⌝.
+
+Definition is_log (v:val) (vs:list Block): iProp Σ :=
+  ∃ (sz: u64) (disk_sz: u64),
+    ⌜v = (#sz, #disk_sz)%V⌝ ∗
+    is_hdr sz disk_sz ∗
+    disk_array 1 vs ∗ ⌜length vs = int.nat sz⌝ ∗
+    (∃ (free: list Block), disk_array (1 + length vs) free ∗
+    ⌜ (1 + length vs + length free)%Z = int.val disk_sz ⌝)
+.
+
+End heap.
