src/go_lang/ffi/disk_prelude.v
@@ -1,6 +1,7 @@
 From Perennial.go_lang Require Import lang.
 From Perennial.go_lang Require ffi.disk.
 Existing Instances disk.disk_op disk.disk_model disk.disk_ty.
+Existing Instances disk.disk_semantics disk.disk_interp.
 Coercion Var' (s: string) := Var s.
 
 Hint Resolve disk.Write_t disk.Read_t disk.Size_t : types.
